\documentclass{article}

\usepackage{listings}
\usepackage[T1]{fontenc}
\usepackage[utf8]{inputenc}
\usepackage{geometry}

\title{Assignment 9}
\date{2019-03-28}
\author{MONTGOMERY, BENNET 20074049 CISC 223\\
		\and GOEL, CHRISTOPHER 20053408 CISC 223\\
		\and VIOLO, JARED 20051382 CISC 223\\
		\and STUART, HARRISON 20067534 CISC 223
		}

\begin{document}
	\maketitle
	
	\section*{Q1}
	\subsection*{(a)}
	First, we apply the modified Hoare axiom scheme process:\\\\
		{\fontfamily{qcr}\selectfont
ASSERT((A | j $\mapsto$ i)[k] >= (A | j $\mapsto$ i)[j])\\
A[j] = A[i];\\
ASSERT(A[k] >= A[j]) //Modified H.A. with previous ASSERT\\\\
	}
	Then we simplify {\fontfamily{qcr}\selectfont P = (A | j $\mapsto$ i)[k] >= (A | j $\mapsto$ i)[j]} with array-componenet substitution notation:\\\\
	{\fontfamily{qcr}\selectfont
		j == k: A[i] >= A[i] //always true\\
		j != k: A[k] >= A[i]\\\\
	}
	Giving us a weakest sufficient precondition\\ {\fontfamily{qcr}\selectfont P = (j == k || A[k] >= A[i])}
	\subsection*{(b)}
	First, we apply the modified Hoare axiom schem process:\\\\
	{\fontfamily{qcr}\selectfont
ASSERT(((A | k $\mapsto$ x) | j $\mapsto$ 2)[i] == 5)\\
A[j] = 2;\\
ASSERT((A | k $\mapsto$ x)[i] == 5) //modified H.A. with previous ASSERT\\ 
A[k] = x;\\
ASSERT(A[i] == 5) //modified H.A. with previous ASSERT\\\\
	}
	Then we simplify {\fontfamily{qcr}\selectfont P = ((A | k $\mapsto$ x) | j $\mapsto$ 2)[i] == 5 } with array-component substitution notation:\\\\
	{\fontfamily{qcr}\selectfont
		k == i: x == 5\\
		k != i: j == i: 2 == 5 //never true\\
		\hphantom{aaaaaaaa} j != i: A[i] == 5\\\\
	}
	Giving us a weakest sufficient precondition\\
	{\fontfamily{qcr}\selectfont
		P = ((k == i \&\& x == 5) || (k != i \&\& j != i \&\& A[i] == 5))
	}
	
	\section*{Q2.}
	The appropriate loop invariant is {\fontfamily{qcr}\selectfont INVAR = ((1 <= j <= n) \&\& ForAll(i = 0; i < j) A[i] == (i + 1) * (i + 2)/2))}. The complete proof tableau is:\\\\
	{\fontfamily{qcr}\selectfont
ASSERT(1 <= n < max)\\
\{ int j; //no effect on logic\\
ASSERT(1 <= 1 <= n \&\& true)\\
\hphantom{aaaa}j = 1;\\
//When j = 1, ForAll statement is 1 == (1)*(2)/2, which evaluates to true\\
ASSERT(1 <= j <= n \&\& ForAll(i = 0; i < j) (A | 0 $\mapsto$ 1)[i] == (i+1)*(i+2)/2)\\
\hphantom{aaaa}A[0] = 1;\\
ASSERT(INVAR) //Modified H.A. with previous ASSERT\\
\hphantom{aaaa}while(j<n) \{\\
ASSERT(INVAR \&\& j < n) //otherwise loop would've terminated\\
//from previous loop iteration\\
ASSERT(ForAll(i = 0; i < j)(A | j $\mapsto$ A[j-1]+j+1)[i] == (i+1)*(i+2)/2)\\
\hphantom{aaaaaaaa}A[j] = A[j-1] + j + 1;\\
ASSERT(ForAll(i = 0; i < j) A[i]  == (i+1)*(i+2)/2) //modified H.A. w/ prev\\
\hphantom{aaaaaaaa}j = j+1;\\
ASSERT(INVAR)\\
\hphantom{aaaa}\}\\
//j == n or loop termination condition would never have been met\\
ASSERT(INVAR \&\& j == n)\\ 
\}\\
//j == n, so we sub n in for j in INVAR\\
ASSERT(ForAll(i = 0; i < n) A[i] == (i+1)*(i+2)/2)
	}
	
\end{document}